main.lean
@@ -1,61 +1,6 @@
-import .int.main  .nat.main
-
-#exit
-import .rev .reify .dnf .scalar .is_lia
-
-open tactic
-
-run_cmd mk_simp_attr `sugar_int 
-attribute [sugar_int] 
-  not_le not_lt
-  int.lt_iff_add_one_le
-  or_false false_or
-  and_true true_and
-  ge gt mul_add add_mul 
-  mul_comm sub_eq_add_neg
-  classical.imp_iff_not_or
-  classical.iff_iff
-
-meta def desugar := `[try {simp only with sugar_int}]
-
-meta def get_polytope : tactic polytope :=
-do `(polytope.unsat %%tsx) ← target, 
-   ts ← eval_expr polytope tsx,
-   return ts
-
-meta def discharge_clause : tactic unit :=
-do ks ← get_polytope >>= scalar.search, 
-   pexpr.apply ``(scalar.unsat_of_unsat_comb %%`(ks) _), 
-   pexpr.apply ``(trivial), skip
-
-meta def discharge_clauses : tactic unit :=
-( pexpr.apply ``(@list.forall_mem_nil (list term) polytope.unsat) >> skip) <|> 
-( do pexpr.apply ``(@list.forall_mem_cons_of (list term) polytope.unsat _ _ _ _), 
-     discharge_clause, discharge_clauses)
-
-lemma uniclo_of_unsat_clausify {p : form} :
-  polytopes.unsat (dnf (¬*p)) → p.uniclo := 
-begin
-  intro h1, 
-  apply uniclo_of_valid,
-  apply valid_of_unsat_not,
-  apply form_unsat_of_polytopes_unsat,
-  assumption,
-end
-
-meta def clausify : tactic unit := 
-pexpr.apply ``(uniclo_of_unsat_clausify _) >> skip
-
-meta def omega_int : tactic unit :=
-do rev_int, desugar, 
-   trace_target,
-   reify, clausify, 
-   discharge_clauses
+import .is_lia .int.main .nat.main
 
 meta def omega : tactic unit := 
-monad.cond is_lia_goal omega_int failed
+monad.cond is_lia_goal int.omega nat.omega 
 
-example (x : int) : 0 ≤ (31 * x) → 0 ≤ x :=
-begin
-  omega,
-end
+
