tests.lean
@@ -17,6 +17,14 @@ meta def ex14 : expr := `(∀ x y : int, x ≤ 3 * y → 3 * x ≤ 9 * y )
 meta def ex15 : expr := `(∀ x : int, (x < 43 ∧ x > 513) → ¬x = x )
 meta def ex16 : expr := `(∀ (x y z w : int), x ≤ y → y ≤ z → z ≤ w → x ≤ w)
 
+meta def ex17 : expr := `(forall (x : nat),  31 * x > 0 → x > 0)
+meta def ex18 : expr := `(forall (x y : nat),  (x ≤ 5 ∧ y ≤ 3) → x + y ≤ 8)
+meta def ex19 : expr := `(forall (x y : nat),  ¬(2 * x + 1 = 2 * y))
+meta def ex20 : expr := `(forall (x y : nat),  x > 0 → x + y > 0)
+meta def ex21 : expr := `(forall (x : nat),  x < 349 ∨ x > 123)
+meta def ex22 : expr := `(forall (x y : nat),  x ≤ 3 * y → 3 * x ≤ 9 * y)
+meta def ex23 : expr := `(forall (x y z : nat), (x ≤ y) → (z > y) → (x - z = 0))
+
 open tactic
 
 meta def BatchTest (slv : tactic unit) : nat → list expr → tactic unit 
@@ -28,10 +36,22 @@ meta def BatchTest (slv : tactic unit) : nat → list expr → tactic unit
     <|> (trace (("Failed ex " : format) ++ format.of_nat idx) >> skip))
     >> BatchTest (idx+1) exps
 
-meta def tests : list expr := 
-[ex01,ex02,ex03,ex04,ex05,ex06,ex07,ex08,ex09,ex10,ex11,ex12,ex13,ex14,ex15,ex16]
+meta def int.tests : list expr := 
+[ex01,ex02,ex03,ex04,ex05,ex06,ex07,ex08,ex09,ex10,
+ ex11,ex12,ex13,ex14,ex15,ex16]
+
+meta def nat.tests : list expr := 
+[ex17,ex18,ex19,ex20,ex21,ex22,ex23]
+
+meta def tests : list expr := int.tests ++ nat.tests
 
 set_option profiler true
+
+example : true := 
+by do BatchTest omega 0 int.tests
+
+example : true := 
+by do BatchTest omega 0 nat.tests
 
 example : true := 
 by do BatchTest omega 0 tests
