int.lean
@@ -1,4 +1,22 @@
-import .list data.int.basic
+import .list data.int.basic .logic
+
+data.int.gcd
+
+namespace int
+
+lemma add_div {a b c : int} : 
+c ∣ a → c ∣ b → (a + b) / c = a / c + b / c :=
+begin
+  intros h1 h2, 
+  by_cases h3 : c = 0,
+  { rw [h3, zero_dvd_iff] at *, 
+    rw [h1, h2, h3], refl },
+  { apply eq_of_mul_eq_mul_right h3,
+    rw add_mul, repeat {rw [int.div_mul_cancel]};
+    try {apply dvd_add}; assumption }
+end
+
+end int
 
 def ints.gcd : list int → nat
 | []      := 0
@@ -28,5 +46,36 @@ if (2 * (i % j)) < j
 then i % j
 else (i % j) - j
 
+lemma symmod_add_one {i} : 
+  0 < i → symmod i (i+1) = -1 := 
+begin
+  intro h1, 
+  simp only [symmod],
+  rw int.mod_eq_of_lt (le_of_lt h1) (lt_add_one _),
+  rw if_neg, simp,
+  have h2 : 2 * i = (1 + 1) * i := rfl,
+  simp [h2, add_mul], apply h1 
+end
 
-#check @dvd_add_iff_left int _
+lemma mul_symdiv_eq {i j} :
+j * (symdiv i j) = i - (symmod i j) := 
+begin
+  simp only [symdiv, symmod],
+  by_cases h1 : (2 * (i % j)) < j,
+  { repeat {rw if_pos h1}, 
+    rw [int.mod_def, sub_sub_cancel] },
+  { repeat {rw if_neg h1},
+    rw [int.mod_def, sub_sub, sub_sub_cancel,
+      mul_add, mul_one] }
+end
+
+lemma symmod_eq {i j} :
+  symmod i j = i - j * (symdiv i j) := 
+by rw [mul_symdiv_eq, sub_sub_cancel]
+
+#exit
+lemma zero_symmod {i} : symmod 0 i = 0 := 
+begin
+  simp only [symmod], 
+  --apply @ite.rec _ _ _ (0 % i) (0 % i - i)  (λ x, x = 0) _ _,
+end
