valuation.lean
@@ -7,10 +7,10 @@ def update (m a) (v : nat → α) : nat → α
 
 notation v `⟨` m `↦` a `⟩` := update m a v
 
-lemma update_eq (m a) (v : nat → α) : update m a v m = a :=
+lemma update_eq (m a) (v : nat → α) : (v ⟨m ↦ a⟩) m = a :=
 begin simp only [update, if_pos rfl] end
 
-lemma update_eq_of_ne {m a} {v : nat → α} {k} : 
+lemma update_eq_of_ne {m a} {v : nat → α} (k) : 
   k ≠ m → update m a v k = v k :=
 begin intro h1, simp only [update], rw if_neg h1 end
 
